feat: (wip) impl `DeBruijn`, pt. 2

Plfl/DeBruijn.lean
@@ -28,25 +28,63 @@ end Ty
 -- https://plfa.github.io/DeBruijn/#contexts
 abbrev Context : Type := List Ty
 
-namespace Context
-  abbrev nil : Context := []
+open List
 
+namespace Context
   abbrev snoc : Context → Ty → Context := flip (· :: ·)
   infixl:50 " :< " => snoc
-
-  abbrev hasMember (ts : Context) (t : Ty) : Prop := t ∈ ts
-  infix:40 " ∋ " => hasMember
 end Context
 
 -- https://plfa.github.io/DeBruijn/#variables-and-the-lookup-judgment
 inductive Lookup : Context → Ty → Type where
 | z : Lookup (Γ :< t) t
 | s : Lookup Γ t → Lookup (Γ :< t') t
+deriving DecidableEq
 
 namespace Lookup
-  example : ∅ :< ℕt =⇒ ℕt :< ℕt ∋ ℕt := by trivial
-  example : ∅ :< ℕt =⇒ ℕt :< ℕt ∋ ℕt =⇒ ℕt := by trivial
+  infix:40 " ∋ " => Lookup
+
+  def getElem {Γ : Context} (n : Fin (Γ.length)) : Γ ∋ Γ[n] :=
+    match Γ, n with
+    | _ :: _, ⟨0, _⟩ => .z
+    | _ :: _, ⟨n + 1, h⟩ => .s (getElem ⟨n, Nat.le_of_succ_le_succ h⟩)
+
+  -- https://github.com/arthurpaulino/lean4-metaprogramming-book/blob/d6a227a63c55bf13d49d443f47c54c7a500ea27b/md/main/macros.md#simplifying-macro-declaration
+  macro " ♯ " n:term:90 : term => `(getElem ⟨$n, by trivial⟩)
+
+  example : ∅ :< ℕt =⇒ ℕt :< ℕt ∋ ℕt := .z
+  example : ∅ :< ℕt =⇒ ℕt :< ℕt ∋ ℕt := ♯0
+  example : ∅ :< ℕt =⇒ ℕt :< ℕt ∋ ℕt =⇒ ℕt := .s .z
+  example : ∅ :< ℕt =⇒ ℕt :< ℕt ∋ ℕt =⇒ ℕt := ♯1
 end Lookup
 
--- Using Elixir notation instead of the native #1...
--- example := &1
+-- https://plfa.github.io/DeBruijn/#terms-and-the-typing-judgment
+/--
+A term with typing judgement embedded in itself.
+-/
+inductive Term : Context → Ty → Type where
+| var : Γ ∋ a → Term Γ a
+| lam : Term (Γ :< a) b → Term Γ (a =⇒ b)
+| ap : Term Γ (a =⇒ b) → Term Γ a → Term Γ b
+| zero : Term Γ ℕt
+| succ : Term Γ ℕt → Term Γ ℕt
+| case : Term Γ ℕt → Term Γ a → Term (Γ :< ℕt) a → Term Γ a
+| mu : Term (Γ :< a) a → Term Γ a
+deriving DecidableEq
+
+namespace Term
+  infix:40 " ⊢ " => Term
+
+  prefix:50 " ƛ " => lam
+  prefix:50 " μ " => mu
+  notation:max " 𝟘? " e " [zero: " o " |succ " n " : " i " ] " => case e o n i
+  infixr:min " $ " => ap
+  infixl:70 " □ " => ap
+  prefix:80 " ι " => succ
+  prefix:90 " ` " => var
+  notation " 𝟘 " => zero
+
+  example : ∅ :< ℕt =⇒ ℕt :< ℕt ⊢ ℕt := `♯0
+  example : ∅ :< ℕt =⇒ ℕt :< ℕt ⊢ ℕt =⇒ ℕt := `♯1
+  example : ∅ :< ℕt =⇒ ℕt :< ℕt ⊢ ℕt := `♯1 □ `♯0
+end Term
